Formalizing disjoint-set forests (union-find).
Hopefully, to prove the functional correctness of the implementation. Then,
convert it to use regions.
- Started writing down a few definitions according following F. Pottier's paper.
- Hit a snag where the [path] relation (reflexive-transitive closure of a
  relation) doesn't work well in a refinement context (can't provide a witness
  for the goal when inside a [Lemma]).
→ about to switch to a constructive style. Hopefully the proofs will go through.

examples/low-level/unification/union-find.fst
@@ -3,7 +3,94 @@
     other-files:ext.fst set.fsi heap.fst st.fst all.fst
   --*)
 module UnionFind
-open FStar.Heap
+
+
+(** 1. Axiomatization of a disjoint set forest (§4 of FP's paper). *)
+
+(* Taken from [metatheory/attic/norm.fst]. See CH's comments in there. *)
+kind Relation (v: Type) = v -> v -> Type
+type path (v: Type) (r: v -> v -> Type): v -> v -> Type =
+  | Refl: x:v -> path v r x x
+  | Step: x:v -> y:v -> z:v -> r x y -> path v r y z -> path v r x z
+
+type is_root (v: Type) (f: Relation v) (x: v) =
+  forall y. ~(f x y)
+type is_repr (v: Type) (f: Relation v) (x: v) (r: v) =
+  path v f x r /\ is_root v f r
+
+type confined (v: Type) (d: Set.set v) (f: Relation v) =
+  forall (x: v) (y: v). path v f x y ==> Set.mem x d /\ Set.mem y d
+type functional (v: Type) (f: Relation v) =
+  forall (x: v) (y: v) (z: v). f x z /\ f y z ==> x = y
+type defined (v: Type) (rel: Relation v) =
+  forall (x: v). exists (r: v). rel x r
+
+type is_dsf (v: Type) (d: Set.set v) (f: Relation v) =
+  confined v d f /\ functional v f /\ defined v (is_repr v f)
+
+(* In FP's development, the following variables are implicit: [v], [f], [x],
+   [z] (and [compress] means [compress v f x z]). *)
+type compress (v: Type) (f: Relation v) (x: v) (z: v) : Relation v =
+  fun (a: v) (b: v) ->
+    (a <> x /\ f a b) \/ (a = x /\ b = z)
+
+
+val compress_preserves_other_edges:
+  v:Type -> f:Relation v -> x:v -> z:v ->
+  u:v -> w:v -> Lemma
+    (requires (f u w /\ u <> x))
+    (ensures (compress v f x z u w))
+let compress_preserves_other_edges (v: Type) (f: Relation v) _ _ _ _ =
+  ()
+
+(* Now [y] is implicit, and [f x y] is implicit too. *)
+val compress_preserves_roots:
+  v:Type -> f:Relation v -> x:v -> y:v -> z:v -> r:v -> Lemma
+    (requires (is_root v f r /\ f x y))
+    (ensures (is_root v (compress v f x z) r))
+let compress_preserves_roots (v: Type) (f: Relation v) _ _ _ _ =
+  ()
+
+
+(* Now [d] is implicit, [is_dsf d f] and [path f y z] too. *)
+val compress_preserves_path_to_roots:
+  v:Type -> d:Set.set v -> f:Relation v ->
+  x:v -> y:v -> z:v ->
+  u:v -> r:v -> #p: path v f u r -> Lemma
+    (requires (f x y /\ path v f y z /\ is_dsf v d f /\ is_root v f r))
+    (ensures (path v (compress v f x z) u r))
+let rec compress_preserves_path_to_roots (v: Type) d (f: Relation v) x y z u r #p =
+  if x = u then begin
+    admit ()
+  end else begin
+    match p with
+    | Refl _ ->
+        assert (u = r);
+        (* JP: I don't understand why F* won't find a proof. *)
+        admit ()
+    | Step _ u' _ _ p' ->
+        compress_preserves_other_edges v f x z u u';
+        assert (compress v f x z u u');
+        (* JP: if I uncomment the line below I get an error for the
+           post-condition of the *entire function*; however, that's very
+           misleading, because I have an admit at the end... *)
+        (* assert (path v f u' r); *)
+        admit ()
+        (* compress_preserves_path_to_roots v d f x y z u' r p';
+        assert (path v (compress v f x z) u' r);
+        admit () *)
+  end
+
+
+val compress_preserves_is_repr:
+  v:Type -> d:Set.set v -> f:Relation v ->
+  x:v -> y:v -> z:v -> u:v -> r:v -> Lemma
+    (requires (is_dsf v d f /\ f x y /\ is_repr v f y z /\ is_repr v f u r))
+    (ensures (is_repr v (compress v f x z) u r))
+let compress_preserves_is_repr (v: Type) d (f: Relation v) x y z u r =
+  compress_preserves_roots v f x y z r;
+  compress_preserves_path_to_roots v d f x y z u r;
+  ()
 
 
 type elem = ref content
